Improve the handling of arithmetic bounds

backends/lean/Base/Primitives.lean
@@ -149,54 +149,78 @@ open System.Platform.getNumBits
 @[simp] def size_num_bits : Nat := (System.Platform.getNumBits ()).val
 
 -- Remark: Lean seems to use < for the comparisons with the upper bounds by convention.
--- We keep the F* convention for now.
-@[simp] def Isize.min : Int := - (HPow.hPow 2 (size_num_bits - 1))
-@[simp] def Isize.max : Int := (HPow.hPow 2 (size_num_bits - 1)) - 1
-@[simp] def I8.min    : Int := - (HPow.hPow 2 7)
-@[simp] def I8.max    : Int := HPow.hPow 2 7 - 1
-@[simp] def I16.min   : Int := - (HPow.hPow 2 15)
-@[simp] def I16.max   : Int := HPow.hPow 2 15 - 1
-@[simp] def I32.min   : Int := -(HPow.hPow 2 31)
-@[simp] def I32.max   : Int := HPow.hPow 2 31 - 1
-@[simp] def I64.min   : Int := -(HPow.hPow 2 63)
-@[simp] def I64.max   : Int := HPow.hPow 2 63 - 1
-@[simp] def I128.min  : Int := -(HPow.hPow 2 127)
-@[simp] def I128.max  : Int := HPow.hPow 2 127 - 1
-@[simp] def Usize.min : Int := 0
-@[simp] def Usize.max : Int := HPow.hPow 2 size_num_bits - 1
-@[simp] def U8.min    : Int := 0
-@[simp] def U8.max    : Int := HPow.hPow 2 8 - 1
-@[simp] def U16.min   : Int := 0
-@[simp] def U16.max   : Int := HPow.hPow 2 16 - 1
-@[simp] def U32.min   : Int := 0
-@[simp] def U32.max   : Int := HPow.hPow 2 32 - 1
-@[simp] def U64.min   : Int := 0
-@[simp] def U64.max   : Int := HPow.hPow 2 64 - 1
-@[simp] def U128.min  : Int := 0
-@[simp] def U128.max  : Int := HPow.hPow 2 128 - 1
 
--- The normalized bounds
-@[simp] def I8.norm_min   := -128
-@[simp] def I8.norm_max   := 127
-@[simp] def I16.norm_min  := -32768
-@[simp] def I16.norm_max  := 32767
-@[simp] def I32.norm_min  := -2147483648
-@[simp] def I32.norm_max  := 2147483647
-@[simp] def I64.norm_min  := -9223372036854775808
-@[simp] def I64.norm_max  := 9223372036854775807
-@[simp] def I128.norm_min := -170141183460469231731687303715884105728
-@[simp] def I128.norm_max := 170141183460469231731687303715884105727
-@[simp] def U8.norm_min   := 0
-@[simp] def U8.norm_max   := 255
-@[simp] def U16.norm_min  := 0
-@[simp] def U16.norm_max  := 65535
-@[simp] def U32.norm_min  := 0
-@[simp] def U32.norm_max  := 4294967295
-@[simp] def U64.norm_min  := 0
-@[simp] def U64.norm_max  := 18446744073709551615
-@[simp] def U128.norm_min := 0
-@[simp] def U128.norm_max := 340282366920938463463374607431768211455
-    
+-- The "structured" bounds
+def Isize.smin : Int := - (HPow.hPow 2 (size_num_bits - 1))
+def Isize.smax : Int := (HPow.hPow 2 (size_num_bits - 1)) - 1
+def I8.smin    : Int := - (HPow.hPow 2 7)
+def I8.smax    : Int := HPow.hPow 2 7 - 1
+def I16.smin   : Int := - (HPow.hPow 2 15)
+def I16.smax   : Int := HPow.hPow 2 15 - 1
+def I32.smin   : Int := -(HPow.hPow 2 31)
+def I32.smax   : Int := HPow.hPow 2 31 - 1
+def I64.smin   : Int := -(HPow.hPow 2 63)
+def I64.smax   : Int := HPow.hPow 2 63 - 1
+def I128.smin  : Int := -(HPow.hPow 2 127)
+def I128.smax  : Int := HPow.hPow 2 127 - 1
+def Usize.smin : Int := 0
+def Usize.smax : Int := HPow.hPow 2 size_num_bits - 1
+def U8.smin    : Int := 0
+def U8.smax    : Int := HPow.hPow 2 8 - 1
+def U16.smin   : Int := 0
+def U16.smax   : Int := HPow.hPow 2 16 - 1
+def U32.smin   : Int := 0
+def U32.smax   : Int := HPow.hPow 2 32 - 1
+def U64.smin   : Int := 0
+def U64.smax   : Int := HPow.hPow 2 64 - 1
+def U128.smin  : Int := 0
+def U128.smax  : Int := HPow.hPow 2 128 - 1
+
+-- The "normalized" bounds, that we use in practice
+def I8.min    := -128
+def I8.max   := 127
+def I16.min  := -32768
+def I16.max  := 32767
+def I32.min  := -2147483648
+def I32.max  := 2147483647
+def I64.min  := -9223372036854775808
+def I64.max  := 9223372036854775807
+def I128.min := -170141183460469231731687303715884105728
+def I128.max := 170141183460469231731687303715884105727
+@[simp] def U8.min   := 0
+def U8.max   := 255
+@[simp] def U16.min  := 0
+def U16.max  := 65535
+@[simp] def U32.min  := 0
+def U32.max  := 4294967295
+@[simp] def U64.min  := 0
+def U64.max  := 18446744073709551615
+@[simp] def U128.min := 0
+def U128.max := 340282366920938463463374607431768211455
+@[simp] def Usize.min := 0
+
+def Isize.refined_min : { n:Int // n = I32.min ∨ n = I64.min } :=
+  ⟨ Isize.smin, by
+    simp [Isize.smin]
+    cases System.Platform.numBits_eq <;>
+    unfold System.Platform.numBits at * <;> simp [*] ⟩
+
+def Isize.refined_max : { n:Int // n = I32.max ∨ n = I64.max } :=
+  ⟨ Isize.smax, by
+    simp [Isize.smax]
+    cases System.Platform.numBits_eq <;>
+    unfold System.Platform.numBits at * <;> simp [*] ⟩
+
+def Usize.refined_max : { n:Int // n = U32.max ∨ n = U64.max } :=
+  ⟨ Usize.smax, by
+    simp [Usize.smax]
+    cases System.Platform.numBits_eq <;>
+    unfold System.Platform.numBits at * <;> simp [*] ⟩
+
+def Isize.min := Isize.refined_min.val
+def Isize.max := Isize.refined_max.val
+def Usize.max := Usize.refined_max.val
+
 inductive ScalarTy :=
 | Isize
 | I8
@@ -210,6 +234,36 @@ inductive ScalarTy :=
 | U32
 | U64
 | U128
+
+def Scalar.smin (ty : ScalarTy) : Int :=
+  match ty with
+  | .Isize => Isize.smin
+  | .I8    => I8.smin
+  | .I16   => I16.smin
+  | .I32   => I32.smin
+  | .I64   => I64.smin
+  | .I128  => I128.smin
+  | .Usize => Usize.smin
+  | .U8    => U8.smin
+  | .U16   => U16.smin
+  | .U32   => U32.smin
+  | .U64   => U64.smin
+  | .U128  => U128.smin
+
+def Scalar.smax (ty : ScalarTy) : Int :=
+  match ty with
+  | .Isize => Isize.smax
+  | .I8    => I8.smax
+  | .I16   => I16.smax
+  | .I32   => I32.smax
+  | .I64   => I64.smax
+  | .I128  => I128.smax
+  | .Usize => Usize.smax
+  | .U8    => U8.smax
+  | .U16   => U16.smax
+  | .U32   => U32.smax
+  | .U64   => U64.smax
+  | .U128  => U128.smax
 
 def Scalar.min (ty : ScalarTy) : Int :=
   match ty with
@@ -241,44 +295,10 @@ def Scalar.max (ty : ScalarTy) : Int :=
   | .U64   => U64.max
   | .U128  => U128.max
 
-@[simp] def Scalar.norm_min (ty : ScalarTy) : Int :=
-  match ty with
-  -- We can't normalize the bounds for isize/usize
-  | .Isize => Isize.min
-  | .Usize => Usize.min
-  --
-  | .I8    => I8.norm_min
-  | .I16   => I16.norm_min
-  | .I32   => I32.norm_min
-  | .I64   => I64.norm_min
-  | .I128  => I128.norm_min
-  | .U8    => U8.norm_min
-  | .U16   => U16.norm_min
-  | .U32   => U32.norm_min
-  | .U64   => U64.norm_min
-  | .U128  => U128.norm_min
-
-@[simp] def Scalar.norm_max (ty : ScalarTy) : Int :=
-  match ty with
-  -- We can't normalize the bounds for isize/usize
-  | .Isize => Isize.max
-  | .Usize => Usize.max
-  --
-  | .I8    => I8.norm_max
-  | .I16   => I16.norm_max
-  | .I32   => I32.norm_max
-  | .I64   => I64.norm_max
-  | .I128  => I128.norm_max
-  | .U8    => U8.norm_max
-  | .U16   => U16.norm_max
-  | .U32   => U32.norm_max
-  | .U64   => U64.norm_max
-  | .U128  => U128.norm_max
-
-def Scalar.norm_min_eq (ty : ScalarTy) : Scalar.min ty = Scalar.norm_min ty := by
+def Scalar.smin_eq (ty : ScalarTy) : Scalar.min ty = Scalar.smin ty := by
   cases ty <;> rfl
 
-def Scalar.norm_max_eq (ty : ScalarTy) : Scalar.max ty = Scalar.norm_max ty := by
+def Scalar.smax_eq (ty : ScalarTy) : Scalar.max ty = Scalar.smax ty := by
   cases ty <;> rfl
 
 -- "Conservative" bounds
@@ -301,30 +321,22 @@ def Scalar.cMax (ty : ScalarTy) : Int :=
 
 theorem Scalar.cMin_bound ty : Scalar.min ty ≤ Scalar.cMin ty := by
   cases ty <;> simp [Scalar.min, Scalar.max, Scalar.cMin, Scalar.cMax] at *
-  cases System.Platform.numBits_eq <;>
-  unfold System.Platform.numBits at * <;>
-  simp [*]
+  have h := Isize.refined_min.property
+  cases h <;> simp [*, Isize.min]
 
 theorem Scalar.cMax_bound ty : Scalar.cMax ty ≤ Scalar.max ty := by
-  cases ty <;> simp [Scalar.min, Scalar.max, Scalar.cMin, Scalar.cMax] at * <;>
-  cases System.Platform.numBits_eq <;>
-  unfold System.Platform.numBits at * <;>
-  simp [*]
+  cases ty <;> simp [Scalar.min, Scalar.max, Scalar.cMin, Scalar.cMax] at *
+  . have h := Isize.refined_max.property
+    cases h <;> simp [*, Isize.max]
+  . have h := Usize.refined_max.property
+    cases h <;> simp [*, Usize.max]
 
 theorem Scalar.cMin_suffices ty (h : Scalar.cMin ty ≤ x) : Scalar.min ty ≤ x := by
-  cases ty <;> simp [Scalar.min, Scalar.max, Scalar.cMin, Scalar.cMax] at * <;>
-  cases System.Platform.numBits_eq <;>
-  unfold System.Platform.numBits at * <;>
-  simp [*] at *
-  -- TODO: I would have expected terms like `-(1 + 1) ^ 63` to be simplified
+  have := Scalar.cMin_bound ty
   linarith
 
 theorem Scalar.cMax_suffices ty (h : x ≤ Scalar.cMax ty) : x ≤ Scalar.max ty := by
-  cases ty <;> simp [Scalar.min, Scalar.max, Scalar.cMin, Scalar.cMax] at * <;>
-  cases System.Platform.numBits_eq <;>
-  unfold System.Platform.numBits at * <;>
-  simp [*] at * <;>
-  -- TODO: I would have expected terms like `-(1 + 1) ^ 63` to be simplified
+  have := Scalar.cMax_bound ty
   linarith
 
 structure Scalar (ty : ScalarTy) where
@@ -609,7 +621,7 @@ def Vec.new (α : Type u): Vec α := ⟨ [], by apply Scalar.cMax_suffices .Usiz
 
 def Vec.len (α : Type u) (v : Vec α) : Usize :=
   let ⟨ v, l ⟩ := v
-  Usize.ofIntCore (List.length v) (by simp [Scalar.min]) l
+  Usize.ofIntCore (List.length v) (by simp [Scalar.min, Usize.min]) l
  
 -- This shouldn't be used
 def Vec.push_fwd (α : Type u) (_ : Vec α) (_ : α) : Unit := ()
@@ -620,13 +632,9 @@ def Vec.push (α : Type u) (v : Vec α) (x : α) : Result (Vec α)
   let nlen := List.length v.val + 1
   if h : nlen ≤ U32.max || nlen ≤ Usize.max then
     have h : nlen ≤ Usize.max := by
-      simp at *
-      cases System.Platform.numBits_eq <;>
-      unfold System.Platform.numBits at * <;>
-      simp [*] at * <;>
-      try assumption
-      cases h <;>
-      linarith
+      simp [Usize.max] at *
+      have hm := Usize.refined_max.property
+      cases h <;> cases hm <;> simp [U32.max, U64.max] at * <;> try linarith
     return ⟨ List.concat v.val x, by simp at *; assumption ⟩
   else
     fail maximumSizeExceeded
@@ -647,7 +655,6 @@ def Vec.insert (α : Type u) (v: Vec α) (i: Usize) (x: α): Result (Vec α) :=
     .ret ⟨ List.set v.val i x, by
       have h: List.length v.val ≤ Usize.max := v.property
       simp [*] at *
-      assumption
     ⟩
   else
     .fail arrayOutOfBounds
@@ -688,7 +695,6 @@ def Vec.index_mut_back (α : Type u) (v: Vec α) (i: Usize) (x: α): Result (Vec
     .ret ⟨ List.set v.val i x, by
       have h: List.length v.val ≤ Usize.max := v.property
       simp [*] at *
-      assumption
     ⟩
   else
     .fail arrayOutOfBounds
